src/Primitive/BooleanExecSpec.v
@@ -18,7 +18,7 @@ Section Decoder.
 Definition bool_decoder td ls : option (bool * Z) :=
     match ls with
     | [] => None
-    | _ => ber_check_tag td ls >>=
+    | _ => ber_check_tags td ls >>=
                         fun x => let c := tag_consumed x in 
                               let e := tag_expected x in 
                               if (Zlength ls - c <? e) || negb (e =? 1) 
