src/Primitive/BooleanVSTSpecDecoder.v
@@ -1,8 +1,9 @@
-Require Import Core.Core Core.StructNormalizer VstLib BooleanExecSpec ErrorWithWriter.
+Require Import Core.Core Core.StructNormalizer
+ VstLib BooleanExecSpec ErrorWithWriter.
 Require Import VST.floyd.proofauto Psatz.
 Require Import VST.floyd.library.
 
-Require Import Clight.BOOLEAN.
+Require Import Clight.BOOLEAN Clight.ber_decoder.
 Require Import StructNormalizer.
 
 
@@ -22,6 +23,40 @@ Definition asn_dec_rval_rep sh v code cons :=
   field_at sh _asn_dec_rval_s_struct 
            [StructField _consumed] 
            (Vint (Int.repr cons)) v)%logic. 
+
+Definition ber_check_tags_spec : ident * funspec :=
+  DECLARE _ber_check_tags
+    WITH (* Codec context pointer *) 
+         sh_ctx : share, ctx_b : block, ctx_ofs : ptrofs, ctx : val,
+         (* Type Descriptor pointer *)
+         sh_td : share, td_b : block, td_ofs : ptrofs, td : TYPE_descriptor,
+         (* Struct context pointer *) 
+         sh_ctx_s : share, ctx_s_b : block, ctx_s_ofs : ptrofs, ctx_s : val,
+         (* Buffer pointer *)
+         sh_ptr : share, ptr_b : block, ptr_ofs : ptrofs, ptr : list byte,
+         (* pointer to the return struct dec_rval *)                        
+         sh_res : share, res_b : block, res_ofs : ptrofs,
+         size : Z, tag_mode : Z, last_tag_from : Z
+         (* sh_ll : share, ll_b : block, ll_ofs : ptrofs, ll : val,
+         sh_opt : share, opt_b : block, opt_ofs : ptrofs, opt : val *)
+
+    PRE [ __res OF (tptr (Tstruct _asn_dec_rval_s noattr)),
+         _opt_codec_ctx OF (tptr (Tstruct _asn_codec_ctx_s noattr)),
+         _td OF (tptr (Tstruct _asn_TYPE_descriptor_s noattr)),
+         _opt_ctx OF (tptr (Tstruct _asn_struct_ctx_s noattr)),
+         _ptr OF (tptr tvoid),
+         _size OF tuint,
+         _tag_mode OF tint,
+         _last_tag_form OF tint,
+         _last_length OF (tptr tint),
+         _opt_tlv_form OF (tptr tint)]
+    PROP ( )
+    LOCAL ()
+    SEP ()
+    POST [tvoid]
+      PROP ()
+      LOCAL ()
+      SEP ().
 
 Definition bool_ber_decode_spec : ident * funspec :=
   DECLARE _BOOLEAN_decode_ber
@@ -85,15 +120,12 @@ Definition bool_ber_decode_spec : ident * funspec :=
                              (default_val (tptr tuchar)) bool_value
            end).
            
-Definition Gprog2 := ltac:(with_library prog [bool_ber_decode_spec]).
+Definition Gprog2 := ltac:(with_library prog [ber_check_tags_spec; bool_ber_decode_spec]).
 
 Theorem bool_der_encode : semax_body Vprog Gprog2 
            (normalize_function f_BOOLEAN_decode_ber composites) bool_ber_decode_spec.
   Proof.
   start_function.
-  unfold MORE_COMMANDS.
-  unfold abbreviate.
-
 Admitted.
 
 End Boolean_ber_decode.
