src/Correctness/BooleanCorrectness.v
@@ -34,7 +34,7 @@ Theorem ber_decoder_correctness : forall td ls b z,
     BER_Bool b (firstn 1 (skipn (Z.to_nat (z - 1)) ls)).
 Proof.
   intros TD ToDec ResB Len DT Dec.
-  unfold bool_decoder, BCTExecSpec.ber_check_tag in Dec; cbn in Dec.
+  unfold bool_decoder, BCTExecSpec.ber_check_tags in Dec; cbn in Dec.
   rewrite DT in Dec; cbn in Dec.
   destruct ToDec eqn:K1; [congruence|]; 
     destruct l eqn:K2; [congruence|]; 
@@ -63,7 +63,7 @@ Proof.
   intros TD ls B z DT Len.
   unfold execErrW, bool_encoder, primitive_encoder, 
   DWTExecSpec.der_write_tags, bool_decoder, 
-  BCTExecSpec.ber_check_tag, bool_of_byte; cbn; rewrite DT.
+  BCTExecSpec.ber_check_tags, bool_of_byte; cbn; rewrite DT.
   intros Res; inversion Res as [T]; clear Res; rename T into Res.
   replace (Byte.repr 1 == 1)%byte with true by reflexivity; cbn.
   replace (Pos.to_nat 2) with (2)%nat by reflexivity.
