src/Lib/BCTVSTSpec.v
@@ -1,0 +1,55 @@
+Require Import Core.Core Core.StructNormalizer
+ VstLib DWTExecSpec ErrorWithWriter BCTExecSpec.
+Require Import VST.floyd.proofauto Psatz.
+Require Import Clight.ber_decoder.
+
+Definition Vprog : varspecs. mk_varspecs prog. Defined.
+Instance CompSpecs : compspecs. make_compspecs prog. Defined.
+
+Open Scope Z.
+
+Section Ber_check_tags.
+
+Definition ber_check_tags_spec : ident * funspec :=
+  DECLARE _ber_check_tags
+    WITH (* Codec context pointer *) 
+         sh_ctx : share, ctx_b : block, ctx_ofs : ptrofs, ctx : val,
+         (* Type Descriptor pointer *)
+         sh_td : share, td_b : block, td_ofs : ptrofs, td : TYPE_descriptor,
+         (* Struct context pointer *) 
+         sh_ctx_s : share, ctx_s_b : block, ctx_s_ofs : ptrofs, ctx_s : val,
+         (* Buffer pointer *)
+         sh_ptr : share, ptr_b : block, ptr_ofs : ptrofs, ptr : list byte,
+         (* pointer to the return struct dec_rval *)                        
+         sh_res : share, res_b : block, res_ofs : ptrofs,
+         size : Z, tag_mode : Z, last_tag_from : Z
+         (* sh_ll : share, ll_b : block, ll_ofs : ptrofs, ll : val,
+         sh_opt : share, opt_b : block, opt_ofs : ptrofs, opt : val *)
+
+    PRE [ __res OF (tptr (Tstruct _asn_dec_rval_s noattr)),
+         _opt_codec_ctx OF (tptr (Tstruct _asn_codec_ctx_s noattr)),
+         _td OF (tptr (Tstruct _asn_TYPE_descriptor_s noattr)),
+         _opt_ctx OF (tptr (Tstruct _asn_struct_ctx_s noattr)),
+         _ptr OF (tptr tvoid),
+         _size OF tuint,
+         _tag_mode OF tint,
+         _last_tag_form OF tint,
+         _last_length OF (tptr tint),
+         _opt_tlv_form OF (tptr tint)]
+    PROP ( )
+    LOCAL ()
+    SEP ()
+    POST [tvoid]
+      PROP ()
+      LOCAL ()
+      SEP ().
+
+Definition Gprog := ltac:(with_library prog [ber_check_tags_spec]).
+
+Theorem bool_der_encode : semax_body Vprog Gprog (normalize_function f_ber_check_tags composites) ber_check_tags_spec.
+Proof.
+  start_function.
+  repeat forward.
+Admitted.
+
+End Ber_check_tags.
